New facilities for automatically proving that functions over lambda-terms are variable-substitution-invariant (that f ([VAR v/u] t) = f t). Clean-up and attempt to get it all to build cleanly once more continues.

examples/lambda/ncLib.sig
@@ -2,8 +2,12 @@ signature ncLib =
 sig
 
   include Abbrev
+  exception ProofFailed of (term list * term) list
+
   val NEW_TAC : string -> term -> tactic
   val NEW_ELIM_TAC : tactic
+  val prove_vsubst_result : thm -> tactic option -> thm
+  val vsubst_tac : thm -> tactic
 
   val recursive_term_function_existence : term -> thm
   val prove_recursive_term_function_exists : term -> thm
